change compile.lem to use finite maps instead of alists
move type definitions out of Lem and into CexpTypesTheory, so that Cv
can be defined manually in HOL.

Correcting compileTermination and beyond to come.

examples/miniML/compiler/CexpTypesScript.sml
@@ -1,5 +1,40 @@
 open HolKernel boolLib bossLib fmaptreeTheory finite_mapTheory pred_setTheory lcsymtacs
-val _ = new_theory"type_Cv"
+val _ = new_theory"CexpTypes"
+
+(* applicative primitives with bytecode counterparts *)
+val _ = Hol_datatype `
+ Cprim2 = CAdd | CSub | CMul | CDiv | CMod | CLt | CEq`;
+
+(* other primitives *)
+val _ = Hol_datatype `
+ Clprim = CLeq | CIf | CAnd | COr`;
+
+
+val _ = Hol_datatype `
+ Cpat =
+    CPvar of string
+  | CPlit of lit
+  | CPcon of num => Cpat list`;
+
+
+val _ = Hol_datatype `
+ Cexp =
+    CDecl of string list
+  | CRaise of error
+  | CVar of string
+  | CLit of lit
+  | CCon of num => Cexp list
+  | CTagEq of Cexp => num
+  | CProj of Cexp => num
+  | CMat of string => (Cpat # Cexp) list
+  | CLet of string list => Cexp list => Cexp
+  | CLetfun of bool => string list => (string list # Cexp) list => Cexp
+  | CFun of string list => Cexp
+  | CCall of Cexp => Cexp list
+  | CPrim2 of Cprim2 => Cexp => Cexp
+  | CLprim of Clprim => Cexp list`;
+
+(* and now the Cv type with its unnecessarily difficult recursion *)
 
 val _ = Parse.overload_on("num_to_s0",``GENLIST (K (CHR 0))``)
 val _ = Parse.overload_on("s0_to_num",``STRLEN``)
@@ -7,8 +42,8 @@ val _ = Parse.overload_on("s0_to_num",``STRLEN``)
 val b = ``:string``
 val a = ``:lit +
 num +
-string list # α +
-string list # (string list # α) list # string``
+string list # Cexp +
+string list # (string list # Cexp) list # string``
 val Cv0 = ``:(^b,^a) fmaptree``
 val _ = Parse.type_abbrev("Cv0",Cv0)
 val Cvwf_def = new_specification("Cvwf_def",["Cvwf"],
@@ -20,29 +55,29 @@ case i of
   | (INR (INL n)) => ∃vs. (fm = FUN_FMAP (combin$C EL vs o s0_to_num) (IMAGE num_to_s0 (count (LENGTH vs))))
   | (INR (INR (INL (xs,b)))) => T
   | (INR (INR (INR (ns,defs,d)))) => T`)
-val Cv1s_exist = new_type_definition("Cv1",
+val Cvs_exist = new_type_definition("Cv",
 prove(
 ``∃v. Cvwf v``,
 qexists_tac`FTNode (INL (Bool F)) FEMPTY` >>
 rw[Cvwf_def]))
 
-val Cv1_bij_thm = define_new_type_bijections {
-  ABS="toCv1", REP="fromCv1", name = "Cv1_bij_thm", tyax = Cv1s_exist}
+val Cv_bij_thm = define_new_type_bijections {
+  ABS="toCv", REP="fromCv", name = "Cv_bij_thm", tyax = Cvs_exist}
 
 val CLitv_def = Define`
-  CLitv l = toCv1 (FTNode (INL l) FEMPTY)`
+  CLitv l = toCv (FTNode (INL l) FEMPTY)`
 val CConv_def = Define`
-  CConv n vs = toCv1
+  CConv n vs = toCv
     (FTNode (INR (INL n))
-            (fromCv1 o_f FUN_FMAP (combin$C EL vs o s0_to_num) (IMAGE num_to_s0 (count (LENGTH vs)))))`
+            (fromCv o_f FUN_FMAP (combin$C EL vs o s0_to_num) (IMAGE num_to_s0 (count (LENGTH vs)))))`
 val CClosure_def = Define`
-  CClosure env xs b = toCv1
+  CClosure env xs b = toCv
     (FTNode (INR (INR (INL (xs,b))))
-            (fromCv1 o_f env))`
+            (fromCv o_f env))`
 val CRecClos_def = Define`
-  CRecClos env ns defs d = toCv1
+  CRecClos env ns defs d = toCv
     (FTNode (INR (INR (INR (ns,defs,d))))
-            (fromCv1 o_f env))`
+            (fromCv o_f env))`
 
 val num_to_s0_inj = store_thm(
 "num_to_s0_inj",
@@ -51,14 +86,14 @@ rpt gen_tac >>
 reverse EQ_TAC >- rw[] >>
 rw[listTheory.LIST_EQ_REWRITE])
 
-val toCv1_thm = store_thm(
-"toCv1_thm",
+val toCv_thm = store_thm(
+"toCv_thm",
 ``Cvwf (FTNode i fm) ⇒
-  (toCv1 (FTNode i fm) = case i of
+  (toCv (FTNode i fm) = case i of
    | INL l => CLitv l
-   | INR (INL n) => CConv n (MAP toCv1 (GENLIST (FAPPLY fm o num_to_s0) (CARD (FDOM fm))))
-   | INR (INR (INL (xs,b))) => CClosure (toCv1 o_f fm) xs b
-   | INR (INR (INR (ns,defs,n))) => CRecClos (toCv1 o_f fm) ns defs n)``,
+   | INR (INL n) => CConv n (MAP toCv (GENLIST (FAPPLY fm o num_to_s0) (CARD (FDOM fm))))
+   | INR (INR (INL (xs,b))) => CClosure (toCv o_f fm) xs b
+   | INR (INR (INR (ns,defs,n))) => CRecClos (toCv o_f fm) ns defs n)``,
 rw[Cvwf_def] >>
 BasicProvers.EVERY_CASE_TAC >- (
   rw[CLitv_def] )
@@ -78,7 +113,7 @@ BasicProvers.EVERY_CASE_TAC >- (
   `num_to_s0 x ∈ IMAGE num_to_s0 (count (LENGTH vs))` by (rw[] >> PROVE_TAC[]) >>
   rw[FUN_FMAP_DEF] >>
   match_mp_tac EQ_SYM >>
-  rw[GSYM (CONJUNCT2 Cv1_bij_thm)] >>
+  rw[GSYM (CONJUNCT2 Cv_bij_thm)] >>
   first_x_assum match_mp_tac >>
   rw[FRANGE_DEF] >>
   qexists_tac `num_to_s0 x` >>
@@ -91,7 +126,7 @@ BasicProvers.EVERY_CASE_TAC >- (
   ONCE_REWRITE_TAC[GSYM fmap_EQ_THM] >>
   rw[] >>
   match_mp_tac EQ_SYM >>
-  rw[GSYM (CONJUNCT2 Cv1_bij_thm)] >>
+  rw[GSYM (CONJUNCT2 Cv_bij_thm)] >>
   first_x_assum match_mp_tac >>
   rw[FRANGE_DEF] >>
   qexists_tac `x` >>
@@ -102,16 +137,16 @@ AP_TERM_TAC >>
 ONCE_REWRITE_TAC[GSYM fmap_EQ_THM] >>
 rw[] >>
 match_mp_tac EQ_SYM >>
-rw[GSYM (CONJUNCT2 Cv1_bij_thm)] >>
+rw[GSYM (CONJUNCT2 Cv_bij_thm)] >>
 first_x_assum match_mp_tac >>
 rw[FRANGE_DEF] >>
 qexists_tac `x` >>
 rw[] )
 
-val Cvwf_all_Cv1 = store_thm(
-"Cvwf_all_Cv1",
-``(∀x. Cvwf x ⇒ P (toCv1 x)) ⇒ (∀v. P v)``,
-metis_tac[Cv1_bij_thm])
+val Cvwf_all_Cv = store_thm(
+"Cvwf_all_Cv",
+``(∀x. Cvwf x ⇒ P (toCv x)) ⇒ (∀v. P v)``,
+metis_tac[Cv_bij_thm])
 
 val Cvwf_thm = LIST_CONJ [
   SIMP_RULE (srw_ss())[](Q.SPEC`INL l`Cvwf_def),
@@ -120,8 +155,8 @@ val Cvwf_thm = LIST_CONJ [
   SIMP_RULE (srw_ss())[](Q.SPEC`INR (INR (INR (ns,defs,n)))`Cvwf_def)
 ]
 
-val Cv1_induction = store_thm(
-"Cv1_induction",
+val Cv_induction = store_thm(
+"Cv_induction",
 ``∀P0 P1 P2.
 (∀l. P0 (CLitv l)) ∧
 (∀vs. P2 vs ⇒ ∀n. P0 (CConv n vs)) ∧
@@ -140,10 +175,10 @@ reverse conj_asm1_tac >- (
     ho_match_mp_tac fmap_INDUCT >>
     rw[] ) >>
   Induct >> rw[]) >>
-match_mp_tac Cvwf_all_Cv1 >>
+match_mp_tac Cvwf_all_Cv >>
 ho_match_mp_tac ft_ind >>
 rpt strip_tac >>
-rw[toCv1_thm] >>
+rw[toCv_thm] >>
 BasicProvers.EVERY_CASE_TAC >- rw[] >>
 first_x_assum match_mp_tac >- (
   `∀vs. EVERY P0 vs ⇒ P2 vs` by (Induct >> rw[]) >>
@@ -193,11 +228,11 @@ qexists_tac `x` >> rw[]
 *)
 )
 
-val toCv1_o_fromCv1 = store_thm(
-"toCv1_o_fromCv1",
-``toCv1 o fromCv1 = I``,
-rw[FUN_EQ_THM,Cv1_bij_thm])
-val _ = export_rewrites["toCv1_o_fromCv1"]
+val toCv_o_fromCv = store_thm(
+"toCv_o_fromCv",
+``toCv o fromCv = I``,
+rw[FUN_EQ_THM,Cv_bij_thm])
+val _ = export_rewrites["toCv_o_fromCv"]
 
 val I_o_f = store_thm(
 "I_o_f",
@@ -205,17 +240,17 @@ val I_o_f = store_thm(
 rw[GSYM fmap_EQ_THM])
 val _ = export_rewrites["I_o_f"]
 
-val Cvwf_fromCv1 = store_thm(
-"Cvwf_fromCv1",
-``∀x. Cvwf (fromCv1 x)``,
-METIS_TAC[Cv1_bij_thm])
-val _ = export_rewrites["Cvwf_fromCv1"]
+val Cvwf_fromCv = store_thm(
+"Cvwf_fromCv",
+``∀x. Cvwf (fromCv x)``,
+METIS_TAC[Cv_bij_thm])
+val _ = export_rewrites["Cvwf_fromCv"]
 
-val Cvwf_o_fromCv1 = store_thm(
-"Cvwf_o_fromCv1",
-``Cvwf o fromCv1 = K T``,
+val Cvwf_o_fromCv = store_thm(
+"Cvwf_o_fromCv",
+``Cvwf o fromCv = K T``,
 rw[FUN_EQ_THM])
-val _ = export_rewrites["Cvwf_o_fromCv1"]
+val _ = export_rewrites["Cvwf_o_fromCv"]
 
 val Cvwf_constructors = store_thm(
 "Cvwf_constructors",
@@ -229,7 +264,7 @@ rw[o_f_FAPPLY] >- (
   `x ∈ FDOM fm` by (
     unabbrev_all_tac >> rw[] >> PROVE_TAC[] ) >>
   rw[o_f_FAPPLY] ) >>
-qexists_tac `MAP fromCv1 vs` >>
+qexists_tac `MAP fromCv vs` >>
 rw[GSYM fmap_EQ_THM] >>
 qmatch_abbrev_tac `X = FUN_FMAP x y ' z` >>
 `z ∈ y` by (
@@ -238,17 +273,17 @@ unabbrev_all_tac >>
 rw[FUN_FMAP_DEF,listTheory.EL_MAP] )
 val _ = export_rewrites["Cvwf_constructors"]
 
-val fromCv1_thm = store_thm(
-"fromCv1_thm",``
-(fromCv1 (CLitv l) = ^(rand(rhs(concl(SPEC_ALL CLitv_def))))) ∧
-(fromCv1 (CConv n vs) = ^(rand(rhs(concl(SPEC_ALL CConv_def))))) ∧
-(fromCv1 (CClosure env xs b) = ^(rand(rhs(concl(SPEC_ALL CClosure_def))))) ∧
-(fromCv1 (CRecClos env ns defs d) = ^(rand(rhs(concl(SPEC_ALL CRecClos_def)))))``,
+val fromCv_thm = store_thm(
+"fromCv_thm",``
+(fromCv (CLitv l) = ^(rand(rhs(concl(SPEC_ALL CLitv_def))))) ∧
+(fromCv (CConv n vs) = ^(rand(rhs(concl(SPEC_ALL CConv_def))))) ∧
+(fromCv (CClosure env xs b) = ^(rand(rhs(concl(SPEC_ALL CClosure_def))))) ∧
+(fromCv (CRecClos env ns defs d) = ^(rand(rhs(concl(SPEC_ALL CRecClos_def)))))``,
 rw[CLitv_def, CConv_def, CClosure_def, CRecClos_def,
-   GSYM (CONJUNCT2 Cv1_bij_thm)])
+   GSYM (CONJUNCT2 Cv_bij_thm)])
 
-val Cv1_Axiom = store_thm(
-"Cv1_Axiom",
+val Cv_Axiom = store_thm(
+"Cv_Axiom",
 ``∀f0 f1 f2 f3 f4 f5 f6.
 ∃fn0 fn1 fn2.
 (∀l. fn0 (CLitv l) = f0 l) ∧
@@ -260,11 +295,11 @@ val Cv1_Axiom = store_thm(
 (∀env. fn2 env = f6 env (fn0 o_f env))``,
 rw[] >>
 qho_match_abbrev_tac `∃fn0. P fn0` >>
-qsuff_tac `∃fn0. P (fn0 o fromCv1)` >- PROVE_TAC[] >>
+qsuff_tac `∃fn0. P (fn0 o fromCv)` >- PROVE_TAC[] >>
 qunabbrev_tac `P` >>
-fs[fromCv1_thm] >>
+fs[fromCv_thm] >>
 qho_match_abbrev_tac `∃fn0 fn1 fn2. P fn0 fn1 fn2` >>
-qsuff_tac `∃fn1 fn0. P fn0 (λvs. fn1 vs (MAP (fn0 o fromCv1) vs)) (λenv. f6 env (fn0 o fromCv1 o_f env))` >- PROVE_TAC[] >>
+qsuff_tac `∃fn1 fn0. P fn0 (λvs. fn1 vs (MAP (fn0 o fromCv) vs)) (λenv. f6 env (fn0 o fromCv o_f env))` >- PROVE_TAC[] >>
 Q.ISPECL_THEN [`λr0:α list. f4`,`λv vs r r0. f5 v vs (HD r0) (r (TL r0))`] strip_assume_tac listTheory.list_Axiom >>
 qexists_tac `fn` >>
 qunabbrev_tac `P` >>
@@ -275,13 +310,13 @@ qexists_tac `fmtreerec
     | (INL l) => f0 l
     | (INR (INL m)) =>
       let vs =
-        (MAP toCv1 (GENLIST (FAPPLY fm o num_to_s0) (CARD (FDOM fm))))
+        (MAP toCv (GENLIST (FAPPLY fm o num_to_s0) (CARD (FDOM fm))))
       in f1 m vs (fn vs (GENLIST (FAPPLY res o num_to_s0) (CARD (FDOM res))))
     | (INR (INR (INL (xs,b)))) =>
-      let env = toCv1 o_f fm in
+      let env = toCv o_f fm in
       f2 env xs b (f6 env res)
     | (INR (INR (INR (ns,defs,d)))) =>
-      let env = toCv1 o_f fm in
+      let env = toCv o_f fm in
       f3 env ns defs d (f6 env res))` >>
 rw[fmtreerec_thm,LET_THM] >>
 rw[listTheory.MAP_GENLIST] >>
@@ -289,7 +324,7 @@ qmatch_abbrev_tac `f1 m vs' (fn vs' gl) = f1 m vs (fn vs ml)` >>
 `vs' = vs` by (
   unabbrev_all_tac >>
   rw[listTheory.LIST_EQ_REWRITE,CARD_INJ_IMAGE,num_to_s0_inj] >>
-  rw[Cv1_bij_thm] >>
+  rw[Cv_bij_thm] >>
   qmatch_abbrev_tac `FUN_FMAP w y ' z = Z` >>
   `z ∈ y` by (
     unabbrev_all_tac >> rw[] >> PROVE_TAC[] ) >>
@@ -302,19 +337,19 @@ unabbrev_all_tac >>
 fs[CARD_INJ_IMAGE,num_to_s0_inj] >>
 rw[listTheory.LIST_EQ_REWRITE,listTheory.EL_MAP] >>
 AP_TERM_TAC >>
-rw[Cv1_bij_thm] >>
+rw[Cv_bij_thm] >>
 AP_TERM_TAC >>
 qmatch_abbrev_tac `FUN_FMAP w y ' z = Z` >>
 `z ∈ y` by (
   unabbrev_all_tac >> rw[] >> PROVE_TAC[] ) >>
 unabbrev_all_tac >>
 rw[FUN_FMAP_DEF] >>
-rw[Cv1_bij_thm])
+rw[Cv_bij_thm])
 
-val [Cv1_case_def] = Prim_rec.define_case_constant Cv1_Axiom
+val [Cv_case_def] = Prim_rec.define_case_constant Cv_Axiom
 
-val Cv1_11 = store_thm(
-"Cv1_11",``
+val Cv_11 = store_thm(
+"Cv_11",``
 (∀l1 l2.
   (CLitv l1 = CLitv l2) = (l1 = l2)) ∧
 (∀m1 vs1 m2 vs2.
@@ -329,20 +364,20 @@ conj_tac >- (
   rw[CLitv_def] >>
   reverse EQ_TAC >- rw[] >>
   strip_tac >>
-  qmatch_assum_abbrev_tac `toCv1 r1 = toCv1 r2` >>
+  qmatch_assum_abbrev_tac `toCv r1 = toCv r2` >>
   `Cvwf r1 ∧ Cvwf r2` by (
     rw[Abbr`r1`,Abbr`r2`] ) >>
-  `r1 = r2` by PROVE_TAC[Cv1_bij_thm] >>
+  `r1 = r2` by PROVE_TAC[Cv_bij_thm] >>
   unabbrev_all_tac >>
   fs[] ) >>
 conj_tac >- (
   rw[CConv_def] >>
   reverse EQ_TAC >- rw[] >>
   strip_tac >>
-  qmatch_assum_abbrev_tac `toCv1 r1 = toCv1 r2` >>
+  qmatch_assum_abbrev_tac `toCv r1 = toCv r2` >>
   `Cvwf r1 ∧ Cvwf r2` by (
     rw[Abbr`r1`,Abbr`r2`]  ) >>
-  `r1 = r2` by PROVE_TAC[Cv1_bij_thm] >>
+  `r1 = r2` by PROVE_TAC[Cv_bij_thm] >>
   unabbrev_all_tac >>
   fsrw_tac[boolSimps.DNF_ss][GSYM fmap_EQ_THM] >>
   fs[IMAGE_11,num_to_s0_inj] >>
@@ -351,33 +386,33 @@ conj_tac >- (
   `num_to_s0 x ∈ IMAGE num_to_s0 (count (LENGTH vs2))` by (
     rw[] >> PROVE_TAC[] ) >>
   rw[FUN_FMAP_DEF] >>
-  PROVE_TAC[Cv1_bij_thm] ) >>
+  PROVE_TAC[Cv_bij_thm] ) >>
 conj_tac >- (
   rw[CClosure_def] >>
   reverse EQ_TAC >- rw[] >>
   strip_tac >>
-  qmatch_assum_abbrev_tac `toCv1 r1 = toCv1 r2` >>
+  qmatch_assum_abbrev_tac `toCv r1 = toCv r2` >>
   `Cvwf r1 ∧ Cvwf r2` by rw[Abbr`r1`,Abbr`r2`] >>
-  `r1 = r2` by PROVE_TAC[Cv1_bij_thm] >>
+  `r1 = r2` by PROVE_TAC[Cv_bij_thm] >>
   unabbrev_all_tac >>
   fsrw_tac[boolSimps.DNF_ss][GSYM fmap_EQ_THM] >>
   pop_assum mp_tac >> rw[] >>
-  PROVE_TAC[Cv1_bij_thm] ) >>
+  PROVE_TAC[Cv_bij_thm] ) >>
 rw[CRecClos_def] >>
 reverse EQ_TAC >- rw[] >>
 strip_tac >>
-qmatch_assum_abbrev_tac `toCv1 r1 = toCv1 r2` >>
+qmatch_assum_abbrev_tac `toCv r1 = toCv r2` >>
 `Cvwf r1 ∧ Cvwf r2` by rw[Abbr`r1`,Abbr`r2`] >>
-`r1 = r2` by PROVE_TAC[Cv1_bij_thm] >>
+`r1 = r2` by PROVE_TAC[Cv_bij_thm] >>
 unabbrev_all_tac >>
 fsrw_tac[boolSimps.DNF_ss][GSYM fmap_EQ_THM] >>
 pop_assum mp_tac >> rw[] >>
-PROVE_TAC[Cv1_bij_thm] )
-val _ = export_rewrites["Cv1_11"]
+PROVE_TAC[Cv_bij_thm] )
+val _ = export_rewrites["Cv_11"]
 
-val Cv1_nice_ind = save_thm(
-"Cv1_nice_ind",
-Cv1_induction
+val Cv_nice_ind = save_thm(
+"Cv_nice_ind",
+Cv_induction
 |> Q.SPECL [`P`,`FEVERY (P o SND)`,`EVERY P`]
 |> SIMP_RULE (srw_ss()) [FEVERY_FEMPTY,FEVERY_STRENGTHEN_THM]
 |> UNDISCH_ALL
@@ -385,22 +420,22 @@ Cv1_induction
 |> DISCH_ALL
 |> Q.GEN `P`)
 
-val Cv1_nchotomy = store_thm(
-"Cv1_nchotomy",
-``∀Cv1.
-  (∃l. Cv1 = CLitv l) ∨
-  (∃m vs. Cv1 = CConv m vs) ∨
-  (∃env xs b. Cv1 = CClosure env xs b) ∨
-  (∃env ns defs n. Cv1 = CRecClos env ns defs n)``,
-ho_match_mp_tac Cv1_nice_ind >> rw[])
+val Cv_nchotomy = store_thm(
+"Cv_nchotomy",
+``∀Cv.
+  (∃l. Cv = CLitv l) ∨
+  (∃m vs. Cv = CConv m vs) ∨
+  (∃env xs b. Cv = CClosure env xs b) ∨
+  (∃env ns defs n. Cv = CRecClos env ns defs n)``,
+ho_match_mp_tac Cv_nice_ind >> rw[])
 
-val Cv1_case_cong = save_thm(
-"Cv1_case_cong",
-Prim_rec.case_cong_thm Cv1_nchotomy Cv1_case_def)
-val _ = DefnBase.export_cong"Cv1_case_cong"
+val Cv_case_cong = save_thm(
+"Cv_case_cong",
+Prim_rec.case_cong_thm Cv_nchotomy Cv_case_def)
+val _ = DefnBase.export_cong"Cv_case_cong"
 
-val Cv1_distinct = store_thm(
-"Cv1_distinct",
+val Cv_distinct = store_thm(
+"Cv_distinct",
 ``(∀l m vs. CLitv l ≠ CConv m vs) ∧
   (∀l env xs b. CLitv l ≠ CClosure env xs b) ∧
   (∀l env ns defs n. CLitv l ≠ CRecClos env ns defs n) ∧
@@ -408,42 +443,41 @@ val Cv1_distinct = store_thm(
   (∀m vs env ns defs n. CConv m vs ≠ CRecClos env ns defs n) ∧
   (∀env xs b envr ns defs n. CClosure env xs b ≠ CRecClos envr ns defs n)``,
 rw[CLitv_def,CConv_def,CClosure_def,CRecClos_def] >>
-qmatch_abbrev_tac `toCv1 r1 ≠ toCv1 r2` >>
-(qsuff_tac `Cvwf r1 ∧ Cvwf r2 ∧ r1 ≠ r2` >- PROVE_TAC[Cv1_bij_thm]) >>
+qmatch_abbrev_tac `toCv r1 ≠ toCv r2` >>
+(qsuff_tac `Cvwf r1 ∧ Cvwf r2 ∧ r1 ≠ r2` >- PROVE_TAC[Cv_bij_thm]) >>
 unabbrev_all_tac >> fs[])
-val _ = export_rewrites["Cv1_distinct"]
+val _ = export_rewrites["Cv_distinct"]
 
 val fmap_size_def = Define`
 fmap_size kz vz fm = SIGMA (λk. kz k + vz (fm ' k)) (FDOM fm)`
 
-val Cv1_size_def =
-Cv1_Axiom
+val Cv_size_def =
+Cv_Axiom
 |> Q.ISPEC `λl. 1 + lit_size l`
-|> Q.ISPEC `λm (vs : β Cv1 list) (r:num). 1 + m + r`
-|> Q.ISPEC `λ(env:string |-> β Cv1) xs (b:β) (r:num). 1 + r + list_size (list_size char_size) xs + Cexp_size b`
-|> Q.ISPEC `λ(env:string |-> β Cv1) ns (defs:(string list,β) env) n r. 1 + r + list_size (list_size char_size) ns + list_size (pair_size (list_size (list_size char_size)) Cexp_size) defs + list_size char_size n`
+|> Q.ISPEC `λm (vs : Cv list) (r:num). 1 + m + r`
+|> Q.ISPEC `λ(env:string |-> Cv) xs b (r:num). 1 + r + list_size (list_size char_size) xs + Cexp_size b`
+|> Q.ISPEC `λ(env:string |-> Cv) ns defs n r. 1 + r + list_size (list_size char_size) ns + list_size (pair_size (list_size (list_size char_size)) Cexp_size) defs + list_size char_size n`
 |> Q.ISPEC `0:num`
-|> Q.ISPEC `λv:β Cv1 (vs : β Cv1 list) (rv:num) rvs. 1 + rv + rvs`
-|> Q.ISPEC `λ(env:string |-> β Cv1). fmap_size (list_size char_size) I`
-|> Q.GEN`Cexp_size`
-|> SIMP_RULE(srw_ss())[SKOLEM_THM]
-|> (fn th => new_specification("Cv1_size_def",["Cv1_size","Cv1s_size","Cv1_env_size"],th))
+|> Q.ISPEC `λv:Cv (vs : Cv list) (rv:num) rvs. 1 + rv + rvs`
+|> Q.ISPEC `λ(env:string |-> Cv). fmap_size (list_size char_size) I`
+|> SIMP_RULE(srw_ss())[]
+|> (fn th => new_specification("Cv_size_def",["Cv_size","Cvs_size","Cv_env_size"],th))
 
 val _ = TypeBase.write
   [TypeBasePure.mk_datatype_info
-     {ax=TypeBasePure.ORIG Cv1_Axiom,
-      case_def=Cv1_case_def,
-      case_cong=Cv1_case_cong,
-      induction=TypeBasePure.ORIG Cv1_induction,
-      nchotomy=Cv1_nchotomy,
-      size=SOME (Parse.Term[QUOTE"Cv1_size"],TypeBasePure.ORIG Cv1_size_def),
+     {ax=TypeBasePure.ORIG Cv_Axiom,
+      case_def=Cv_case_def,
+      case_cong=Cv_case_cong,
+      induction=TypeBasePure.ORIG Cv_induction,
+      nchotomy=Cv_nchotomy,
+      size=SOME (Parse.Term[QUOTE"Cv_size"],TypeBasePure.ORIG Cv_size_def),
       encode=NONE,
       fields=[], accessors=[], updates=[],
       recognizers = [],
       destructors = [],
       lift=NONE,
-      one_one=SOME Cv1_11,
-      distinct=SOME Cv1_distinct}];
+      one_one=SOME Cv_11,
+      distinct=SOME Cv_distinct}];
 
 val _ = adjoin_to_theory
 {sig_ps = NONE,
@@ -453,18 +487,18 @@ val _ = adjoin_to_theory
    in
 S "val _ = TypeBase.write"                          ;NL();
 S "  [TypeBasePure.mk_datatype_info"                ;NL();
-S "     {ax=TypeBasePure.ORIG Cv1_Axiom,"           ;NL();
-S "      case_def=Cv1_case_def,"                    ;NL();
-S "      case_cong=Cv1_case_cong,"                  ;NL();
-S "      induction=TypeBasePure.ORIG Cv1_induction,";NL();
-S "      nchotomy=Cv1_nchotomy,"                    ;NL();
-S "      size=SOME (Parse.Term[QUOTE\"Cv1_size\"],TypeBasePure.ORIG Cv1_size_def),";NL();
+S "     {ax=TypeBasePure.ORIG Cv_Axiom,"           ;NL();
+S "      case_def=Cv_case_def,"                    ;NL();
+S "      case_cong=Cv_case_cong,"                  ;NL();
+S "      induction=TypeBasePure.ORIG Cv_induction,";NL();
+S "      nchotomy=Cv_nchotomy,"                    ;NL();
+S "      size=SOME (Parse.Term[QUOTE\"Cv_size\"],TypeBasePure.ORIG Cv_size_def),";NL();
 S "      encode=NONE,"                              ;NL();
 S "      fields=[], accessors=[], updates=[],"      ;NL();
 S "      recognizers = [],"                         ;NL();
 S "      destructors = [],"                         ;NL();
 S "      lift=NONE,"                                ;NL();
-S "      one_one=SOME Cv1_11,"                      ;NL();
-S "      distinct=SOME Cv1_distinct}];"             ;NL()end)}
+S "      one_one=SOME Cv_11,"                      ;NL();
+S "      distinct=SOME Cv_distinct}];"             ;NL()end)}
 
 val _ = export_theory()
